new/golang/theory/intoval.v
@@ -8,30 +8,34 @@ Set Default Proof Mode "Classic".
 From New.golang.defn Require Export postlang.
 
 Section defs.
-(** Proven (i.e. untrusted) definitions and properties associated with types `V`
-    that have an `IntoVal` instance. *)
-Class IntoValProof (V : Type) `{IntoVal V} :=
+
+Context `{sem: ffi_semantics} `{!ffi_interp ffi} `{!heapGS Σ}.
+
+Class IntoValComparable (V : Type) `{!IntoVal V} :=
   {
-    typed_pointsto_def `{sem: ffi_semantics} `{!ffi_interp ffi} `{!heapGS Σ}
-      (l : loc) (dq : dfrac) (v : V) : iProp Σ;
     #[global] to_val_inj :: Inj (=) (=) (to_val (V:=V));
     #[global] to_val_eqdec :: EqDecision V ;
   }.
+
+Class TypedPointsto (V : Type) `{!IntoVal V} :=
+{
+  typed_pointsto_def (l : loc) (dq : dfrac) (v : V) : iProp Σ
+}.
+
 Program Definition typed_pointsto := sealed @typed_pointsto_def.
 Definition typed_pointsto_unseal : typed_pointsto = _ := seal_eq _.
-Arguments typed_pointsto {_ _ _ _ _ _ _ _ _ _} (l dq v).
+Global Arguments typed_pointsto {_ _ _} (l dq v).
 Notation "l ↦ dq v" := (typed_pointsto l dq v%V)
                          (at level 20, dq custom dfrac at level 1,
                             format "l  ↦ dq  v") : bi_scope.
 
-Context `{sem: ffi_semantics} `{!ffi_interp ffi} `{!heapGS Σ}.
 (** [IntoValTyped V t] provides proofs that loading and storing [t] respects
     the typed points-to for `V`.
 
     [typed_pointsto_def] is in [IntoValProof] rather than here because `l ↦ v`
     not explicitly mention `t`, and there can be multiple `t`s for a single `V`
     (e.g. int64 and uint64 both have w64). *)
-Class IntoValTyped (V : Type) (t : go.type) `{!IntoVal V} `{!IntoValProof V} :=
+Class IntoValTyped (V : Type) (t : go.type) `{TypedPointsto V} :=
   {
     wp_load : (∀ l dq (v : V), {{{ l ↦{dq} v }}}
                                  load t #l
@@ -43,3 +47,7 @@ Class IntoValTyped (V : Type) (t : go.type) `{!IntoVal V} `{!IntoValProof V} :=
 (* [t] should not be an evar before doing typeclass search *)
 Global Hint Mode IntoValTyped - ! - - : typeclass_instances.
 End defs.
+
+Notation "l ↦ dq v" := (typed_pointsto l dq v%V)
+                         (at level 20, dq custom dfrac at level 1,
+                            format "l  ↦ dq  v") : bi_scope.
